simulation/correct_step_opcode_alu32.v
@@ -9,16 +9,18 @@ From bpf.proof Require Import Clightlogic MatchState CorrectRel CommonLemma Comm
 
 From bpf.clight Require Import interpreter.
 
-From bpf.simulation Require Import correct_get_opcode_alu64 correct_upd_reg correct_upd_flag correct_reg64_to_reg32.
+From bpf.simulation Require Import correct_get_opcode_alu32 correct_upd_reg correct_upd_flag correct_reg64_to_reg32.
+
+
 (**
-Check step_opcode_alu64.
-step_opcode_alu64
-     : val64_t -> val64_t -> DxRegs.reg -> int8_t -> M unit
+Check step_opcode_alu32.
+step_opcode_alu32
+     : val -> val -> reg -> nat -> M unit
 
 *)
 Open Scope Z_scope.
 
-Section Step_opcode_alu64.
+Section Step_opcode_alu32.
 
   (** The program contains our function of interest [fn] *)
   Definition p : Clight.program := prog.
@@ -29,7 +31,7 @@ Section Step_opcode_alu64.
   Definition res : Type := unit.
 
   (* [f] is a Coq Monadic function with the right type *)
-  Definition f : arrow_type args (M res) := step_opcode_alu64.
+  Definition f : arrow_type args (M res) := step_opcode_alu32.
 
   Variable state_block: block. (**r a block storing all rbpf state information? *)
   Variable mrs_block: block.
@@ -41,13 +43,13 @@ Section Step_opcode_alu64.
     v = Vptr state_block Ptrofs.zero /\ match_state state_block mrs_block ins_block stm m.
 
   (* [fn] is the Cligth function which has the same behaviour as [f] *)
-  Definition fn: Clight.function := f_step_opcode_alu64.
+  Definition fn: Clight.function := f_step_opcode_alu32.
 
   (* [match_arg] relates the Coq arguments and the C arguments *)
   Definition match_arg_list : DList.t (fun x => x -> val -> State.state -> Memory.Mem.mem -> Prop) ((unit:Type) ::args) :=
     (DList.DCons stateM_correct
-      (DList.DCons (stateless val64_correct)
-       (DList.DCons (stateless val64_correct)
+      (DList.DCons (stateless valu32_correct)
+       (DList.DCons (stateless valu32_correct)
           (DList.DCons (stateless reg_correct)
             (DList.DCons (stateless opcode_correct)
                     (DList.DNil _)))))).
@@ -78,22 +80,14 @@ Ltac correct_forward L :=
       eapply correct_statement_if_body; [prove_in_inv | destruct x ]
   end.
 
-  Lemma Cop_add : forall vl1 vl2 m,
-       Cop.sem_binary_operation (globalenv p) Cop.Oadd
-                                (Vlong vl1) Clightdefs.tulong (Vlong vl2) Clightdefs.tulong m =
-         Some (Vlong (Int64.add vl1 vl2)).
-  Proof.
-    reflexivity.
-  Qed.
-
-  Instance correct_function3_step_opcode_alu64 : forall a, correct_function3 p args res f fn modifies false match_arg_list match_res a.
+  Instance correct_function3_step_opcode_alu32 : forall a, correct_function3 p args res f fn modifies false match_arg_list match_res a.
   Proof.
     correct_function_from_body args.
     correct_body.
 
-    unfold f, step_opcode_alu64.
+    unfold f, step_opcode_alu32.
     simpl.
-    (** goal: correct_body _ _ (bindM (get_opcode_alu64 _) ... *)
+    (** goal: correct_body _ _ (bindM (get_opcode_alu32 _) ... *)
     correct_forward correct_statement_seq_body_nil.
 
     my_reflex.
@@ -131,11 +125,11 @@ Ltac correct_forward L :=
 
     (** goal: correct_body _ _
               match x with
-              | op_BPF_ADD64 => bindM (upd_reg ... *)
+              | op_BPF_ADD32 => bindM (upd_reg ... *)
     intros.
     unfold INV.
-    destruct x eqn: Halu. (**r case discussion on each alu64_instruction *)
-    - (**r op_BPF_ADD64 *)
+    destruct x eqn: Halu. (**r case discussion on each alu32_instruction *)
+    - (**r op_BPF_ADD32 *)
       eapply correct_statement_switch with (n:= 0).
       + simpl.
         (**r s1 -> (Ssequence s1 s2) *)
@@ -184,27 +178,27 @@ Ltac correct_forward L :=
         correct_Forall.
         get_invariant _st.
         get_invariant _dst.
-        get_invariant _dst64.
-        get_invariant _src64.
-        unfold val64_correct,stateless in c5, c6.
+        get_invariant _dst32.
+        get_invariant _src32.
+        unfold valu32_correct,stateless in c5, c6.
         destruct c5 as (Hv1_eq & (vl1 & Hvl1_eq)); subst.
         destruct c6 as (Hv2_eq & (vl2 & Hvl2_eq)); subst.
-        exists (v ::v0 :: Vlong (Int64.add vl1 vl2) :: nil).
+        exists (v ::v0 :: Vlong (Int64.repr (Int.unsigned (Int.add vl1 vl2))) :: nil). (**r star here *)
         unfold map_opt, exec_expr.
-        rewrite p0.
-        rewrite p1. rewrite p2. rewrite p3.
-        split.
-        reflexivity.
-        intros.
-        simpl.
+        rewrite p0, p1, p2, p3.
+        unfold Cop.sem_binary_operation.
+        unfold Cop.sem_add.
+        unfold Cop.classify_add, typeof; simpl.
+        split; [reflexivity | ].
+        intros; simpl.
         intuition.
         unfold stateless,val64_correct.
-        split; auto. eexists ; reflexivity.
+        split; [reflexivity | eexists ; reflexivity].
         intros.
 
         (**r goal: correct_body p unit (returnM tt) fn (Sreturn None) modifies *)
         eapply correct_body_Sreturn_None. (** from `upd_flag DxFlag.BPF_OK` to `bindM (upd_flag DxFlag.BPF_OK) returnM` *)
-        unfold match_res, correct_get_opcode_alu64.match_res.
+        unfold match_res, correct_get_opcode_alu32.match_res.
         intros.
         get_invariant _st.
         unfold stateM_correct in c3.
@@ -212,15 +206,15 @@ Ltac correct_forward L :=
         reflexivity.
       + reflexivity.
       + intros.
-        get_invariant _opcode_alu64.
+        get_invariant _opcode_alu32.
         unfold exec_expr.
         rewrite p0. f_equal.
-        unfold correct_get_opcode_alu64.match_res in c3.
-        unfold opcode_alu64_correct in c3.
-        (* opcode_alu64_correct should be a mapping between opcodes and int *)
+        unfold correct_get_opcode_alu32.match_res in c3.
+        unfold opcode_alu32_correct in c3.
+        (* opcode_alu32_correct should be a mapping between opcodes and int *)
         destruct c3; assumption.
       + compute. intuition congruence.
-    - (**r op_BPF_SUB64 *)
+    - (**r op_BPF_SUB32 *)
       eapply correct_statement_switch with (n:= 16).
       + simpl.
         (**r s1 -> (Ssequence s1 s2) *)
@@ -269,27 +263,26 @@ Ltac correct_forward L :=
         correct_Forall.
         get_invariant _st.
         get_invariant _dst.
-        get_invariant _dst64.
-        get_invariant _src64.
-        unfold val64_correct,stateless in c5, c6.
+        get_invariant _dst32.
+        get_invariant _src32.
+        unfold valu32_correct,stateless in c5, c6.
         destruct c5 as (Hv1_eq & (vl1 & Hvl1_eq)); subst.
         destruct c6 as (Hv2_eq & (vl2 & Hvl2_eq)); subst.
-        exists (v ::v0 :: Vlong (Int64.sub vl1 vl2) :: nil). (**r star here *)
+        exists (v ::v0 :: Vlong (Int64.repr (Int.unsigned (Int.sub vl1 vl2))) :: nil). (**r star here *)
         unfold map_opt, exec_expr.
-        rewrite p0.
-        rewrite p1. rewrite p2. rewrite p3.
-        split.
-        reflexivity.
-        intros.
-        simpl.
+        rewrite p0, p1, p2, p3.
+        unfold Cop.sem_binary_operation, typeof.
+        unfold Cop.sem_sub, Cop.classify_sub; simpl.
+        split; [reflexivity | ].
+        intros; simpl.
         intuition.
         unfold stateless,val64_correct.
-        split; auto. eexists ; reflexivity.
+        split; [reflexivity | eexists ; reflexivity].
         intros.
 
         (**r goal: correct_body p unit (returnM tt) fn (Sreturn None) modifies *)
         eapply correct_body_Sreturn_None.
-        unfold match_res, correct_get_opcode_alu64.match_res.
+        unfold match_res, correct_get_opcode_alu32.match_res.
         intros.
         get_invariant _st.
         unfold stateM_correct in c3.
@@ -297,15 +290,15 @@ Ltac correct_forward L :=
         reflexivity.
       + reflexivity.
       + intros.
-        get_invariant _opcode_alu64.
+        get_invariant _opcode_alu32.
         unfold exec_expr.
         rewrite p0. f_equal.
-        unfold correct_get_opcode_alu64.match_res in c3.
-        unfold opcode_alu64_correct in c3.
-        (* opcode_alu64_correct should be a mapping between opcodes and int *)
+        unfold correct_get_opcode_alu32.match_res in c3.
+        unfold opcode_alu32_correct in c3.
+        (* opcode_alu32_correct should be a mapping between opcodes and int *)
         destruct c3; assumption.
       + compute. intuition congruence.
-    - (**r op_BPF_MUL64 *)
+    - (**r op_BPF_MUL32 *)
       eapply correct_statement_switch with (n:= 32).
       + simpl.
         (**r s1 -> (Ssequence s1 s2) *)
@@ -354,27 +347,26 @@ Ltac correct_forward L :=
         correct_Forall.
         get_invariant _st.
         get_invariant _dst.
-        get_invariant _dst64.
-        get_invariant _src64.
-        unfold val64_correct,stateless in c5, c6.
+        get_invariant _dst32.
+        get_invariant _src32.
+        unfold valu32_correct,stateless in c5, c6.
         destruct c5 as (Hv1_eq & (vl1 & Hvl1_eq)); subst.
         destruct c6 as (Hv2_eq & (vl2 & Hvl2_eq)); subst.
-        exists (v ::v0 :: Vlong (Int64.mul vl1 vl2) :: nil). (**r star here *)
+        exists (v ::v0 :: Vlong (Int64.repr (Int.unsigned (Int.mul vl1 vl2))) :: nil). (**r star here *)
         unfold map_opt, exec_expr.
-        rewrite p0.
-        rewrite p1. rewrite p2. rewrite p3.
-        split.
-        reflexivity.
-        intros.
-        simpl.
+        rewrite p0, p1, p2, p3.
+        unfold Cop.sem_binary_operation, typeof.
+        unfold Cop.sem_mul, Cop.sem_binarith; simpl.
+        split; [reflexivity | ].
+        intros; simpl.
         intuition.
         unfold stateless,val64_correct.
-        split; auto. eexists ; reflexivity.
+        split; [reflexivity | eexists ; reflexivity].
         intros.
 
         (**r goal: correct_body p unit (returnM tt) fn (Sreturn None) modifies *)
         eapply correct_body_Sreturn_None.
-        unfold match_res, correct_get_opcode_alu64.match_res.
+        unfold match_res, correct_get_opcode_alu32.match_res.
         intros.
         get_invariant _st.
         unfold stateM_correct in c3.
@@ -382,23 +374,28 @@ Ltac correct_forward L :=
         reflexivity.
       + reflexivity.
       + intros.
-        get_invariant _opcode_alu64.
+        get_invariant _opcode_alu32.
         unfold exec_expr.
         rewrite p0. f_equal.
-        unfold correct_get_opcode_alu64.match_res in c3.
-        unfold opcode_alu64_correct in c3.
-        (* opcode_alu64_correct should be a mapping between opcodes and int *)
+        unfold correct_get_opcode_alu32.match_res in c3.
+        unfold opcode_alu32_correct in c3.
+        (* opcode_alu32_correct should be a mapping between opcodes and int *)
         destruct c3; assumption.
       + compute. intuition congruence.
-    - (**r op_BPF_DIV64 *)
+    - (**r op_BPF_DIV32 *)
       eapply correct_statement_switch with (n:= 48).
       + simpl.
         (**r s1 -> (Ssequence s1 s2) *)
         eapply correct_statement_seq_body_drop.
         intros.
-        (**r correct_body p unit (if rBPFValues.compl_ne c0 val64_zero then ... *)
+        (**r correct_body p unit (if rBPFValues.compl_ne c0 val32_zero then ... *)
         eapply correct_statement_if_body_expr.
-        destruct (rBPFValues.compl_ne c0 (Vlong Int64.zero)) eqn: Hdiv_zero.
+        change Vzero with (Vint Int.zero).
+        unfold rBPFValues.comp_ne_32.
+        destruct (match c0 with
+                  | Vint n1 => negb (Int.eq n1 Int.zero)
+                  | _ => false
+                  end) eqn: Hdiv_zero.
 
 
         eapply correct_statement_seq_body_unit.
@@ -443,44 +440,39 @@ Ltac correct_forward L :=
         correct_Forall.
         get_invariant _st.
         get_invariant _dst.
-        get_invariant _dst64.
-        get_invariant _src64.
-        unfold val64_correct,stateless in c5, c6.
+        get_invariant _dst32.
+        get_invariant _src32.
+        unfold valu32_correct,stateless in c5, c6.
         destruct c5 as (Hv1_eq & (vl1 & Hvl1_eq)); subst.
         destruct c6 as (Hv2_eq & (vl2 & Hvl2_eq)); subst.
-        unfold rBPFValues.val64_divlu, Val.divlu. (**r star here *)
-        unfold rBPFValues.compl_ne in Hdiv_zero.
+        unfold rBPFValues.val32_divu, Val.divlu. (**r star here *)
         rewrite Bool.negb_true_iff in Hdiv_zero.
-        rewrite Hdiv_zero.
-        exists (v ::v0 :: Vlong (Int64.divu vl1 vl2) :: nil). (**r star here *)
+        
+        exists (v ::v0 :: Vlong (Int64.repr (Int.unsigned (Int.divu vl1 vl2))) :: nil). (**r star here *)
         unfold map_opt, exec_expr.
-        rewrite p0.
-        rewrite p1. rewrite p2. rewrite p3.
-        split.
-        simpl.
-        unfold Cop.sem_div, Cop.sem_binarith;
-        simpl.
-        Transparent Archi.ptr64.
-        unfold Cop.sem_cast; simpl.
+        rewrite p0, p1, p2, p3.
+        unfold Cop.sem_binary_operation, typeof.
+        unfold Cop.sem_div, Cop.sem_binarith; simpl.
         rewrite Hdiv_zero.
-        reflexivity.
-        intros.
-        simpl.
+        unfold Cop.sem_cast; simpl.
+        split; [reflexivity | ].
+        intros; simpl.
         intuition.
         unfold stateless,val64_correct.
-        split; auto. eexists ; reflexivity.
+        split; [reflexivity | eexists ; reflexivity].
         intros.
 
         (**r goal: correct_body p unit (returnM tt) fn (Sreturn None) modifies *)
         eapply correct_body_Sreturn_None.
-        unfold match_res, correct_get_opcode_alu64.match_res.
+        unfold match_res, correct_get_opcode_alu32.match_res.
         intros.
         get_invariant _st.
         unfold stateM_correct in c3.
         destruct c3 as (_ & c3); assumption.
         reflexivity.
 
-        unfold rBPFValues.compl_ne, val64_zero in Hdiv_zero.
+        change (upd_flag Flag.BPF_ILLEGAL_DIV) with
+          (bindM (upd_flag Flag.BPF_ILLEGAL_DIV) (fun _ : unit => returnM tt)).
         (**r goal: correct_body p unit (upd_flag Flag.BPF_ILLEGAL_DIV) fn ... *)
         eapply correct_statement_seq_body_unit.
         change_app_for_statement.
@@ -524,9 +516,9 @@ Ltac correct_forward L :=
         correct_Forall.
         get_invariant _st.
         get_invariant _dst.
-        get_invariant _dst64.
-        get_invariant _src64.
-        unfold val64_correct,stateless in c5, c6.
+        get_invariant _dst32.
+        get_invariant _src32.
+        unfold valu32_correct,stateless in c5, c6.
         destruct c5 as (Hv1_eq & (vl1 & Hvl1_eq)); subst.
         destruct c6 as (Hv2_eq & (vl2 & Hvl2_eq)); subst.
         exists (v ::Vint (Int.neg (Int.repr 9)) :: nil). (**r star here *)
@@ -538,13 +530,13 @@ Ltac correct_forward L :=
         intros.
         simpl.
         intuition.
-        unfold stateless,val64_correct.
+        unfold stateless,valu32_correct.
         split; auto.
         intros.
 
         (**r goal: correct_body p unit (returnM tt) fn (Sreturn None) modifies *)
         eapply correct_body_Sreturn_None.
-        unfold match_res, correct_get_opcode_alu64.match_res.
+        unfold match_res, correct_get_opcode_alu32.match_res.
         intros.
         get_invariant _st.
         unfold stateM_correct in c3.
@@ -553,26 +545,26 @@ Ltac correct_forward L :=
         reflexivity.
 
         intros.
-        get_invariant _src64.
+        get_invariant _src32.
         unfold exec_expr.
-        rewrite p0. unfold val64_zero, rBPFValues.compl_ne, Int64.zero.
+        rewrite p0. unfold Vzero, rBPFValues.comp_ne_32, Int.zero.
         unfold Cop.sem_binary_operation, Cop.sem_cmp, Cop.sem_binarith, Cop.sem_cast; simpl.
-        unfold stateless, val64_correct in c3.
+        unfold stateless, valu32_correct in c3.
         destruct c3 as (c3_0 & c3_vl & c3_1).
         subst.
         reflexivity.
 
       + reflexivity.
       + intros.
-        get_invariant _opcode_alu64.
+        get_invariant _opcode_alu32.
         unfold exec_expr.
         rewrite p0. f_equal.
-        unfold correct_get_opcode_alu64.match_res in c3.
-        unfold opcode_alu64_correct in c3.
-        (* opcode_alu64_correct should be a mapping between opcodes and int *)
+        unfold correct_get_opcode_alu32.match_res in c3.
+        unfold opcode_alu32_correct in c3.
+        (* opcode_alu32_correct should be a mapping between opcodes and int *)
         destruct c3; assumption.
       + compute. intuition congruence.
-    - (**r op_BPF_OR64 *)
+    - (**r op_BPF_OR32 *)
       eapply correct_statement_switch with (n:= 64).
       + simpl.
         (**r s1 -> (Ssequence s1 s2) *)
@@ -621,27 +613,26 @@ Ltac correct_forward L :=
         correct_Forall.
         get_invariant _st.
         get_invariant _dst.
-        get_invariant _dst64.
-        get_invariant _src64.
-        unfold val64_correct,stateless in c5, c6.
+        get_invariant _dst32.
+        get_invariant _src32.
+        unfold valu32_correct,stateless in c5, c6.
         destruct c5 as (Hv1_eq & (vl1 & Hvl1_eq)); subst.
         destruct c6 as (Hv2_eq & (vl2 & Hvl2_eq)); subst.
-        exists (v ::v0 :: Vlong (Int64.or vl1 vl2) :: nil). (**r star here *)
+        exists (v ::v0 :: Vlong (Int64.repr (Int.unsigned (Int.or vl1 vl2))) :: nil). (**r star here *)
         unfold map_opt, exec_expr.
-        rewrite p0.
-        rewrite p1. rewrite p2. rewrite p3.
-        split.
-        reflexivity.
-        intros.
-        simpl.
+        rewrite p0, p1, p2, p3.
+        unfold Cop.sem_binary_operation, typeof.
+        unfold Cop.sem_or, Cop.sem_binarith; simpl.
+        split; [reflexivity | ].
+        intros; simpl.
         intuition.
         unfold stateless,val64_correct.
-        split; auto. eexists ; reflexivity.
+        split; [reflexivity | eexists ; reflexivity].
         intros.
 
         (**r goal: correct_body p unit (returnM tt) fn (Sreturn None) modifies *)
         eapply correct_body_Sreturn_None.
-        unfold match_res, correct_get_opcode_alu64.match_res.
+        unfold match_res, correct_get_opcode_alu32.match_res.
         intros.
         get_invariant _st.
         unfold stateM_correct in c3.
@@ -649,12 +640,12 @@ Ltac correct_forward L :=
         reflexivity.
       + reflexivity.
       + intros.
-        get_invariant _opcode_alu64.
+        get_invariant _opcode_alu32.
         unfold exec_expr.
         rewrite p0. f_equal.
-        unfold correct_get_opcode_alu64.match_res in c3.
-        unfold opcode_alu64_correct in c3.
-        (* opcode_alu64_correct should be a mapping between opcodes and int *)
+        unfold correct_get_opcode_alu32.match_res in c3.
+        unfold opcode_alu32_correct in c3.
+        (* opcode_alu32_correct should be a mapping between opcodes and int *)
         destruct c3; assumption.
       + compute. intuition congruence.
     - (**r op_BPF_AND64 *)
@@ -706,27 +697,26 @@ Ltac correct_forward L :=
         correct_Forall.
         get_invariant _st.
         get_invariant _dst.
-        get_invariant _dst64.
-        get_invariant _src64.
-        unfold val64_correct,stateless in c5, c6.
+        get_invariant _dst32.
+        get_invariant _src32.
+        unfold valu32_correct,stateless in c5, c6.
         destruct c5 as (Hv1_eq & (vl1 & Hvl1_eq)); subst.
         destruct c6 as (Hv2_eq & (vl2 & Hvl2_eq)); subst.
-        exists (v ::v0 :: Vlong (Int64.and vl1 vl2) :: nil). (**r star here *)
+        exists (v ::v0 :: Vlong (Int64.repr (Int.unsigned (Int.and vl1 vl2))) :: nil). (**r star here *)
         unfold map_opt, exec_expr.
-        rewrite p0.
-        rewrite p1. rewrite p2. rewrite p3.
-        split.
-        reflexivity.
-        intros.
-        simpl.
+        rewrite p0, p1, p2, p3.
+        unfold Cop.sem_binary_operation, typeof.
+        unfold Cop.sem_and, Cop.sem_binarith; simpl.
+        split; [reflexivity | ].
+        intros; simpl.
         intuition.
         unfold stateless,val64_correct.
-        split; auto. eexists ; reflexivity.
+        split; [reflexivity | eexists ; reflexivity].
         intros.
 
         (**r goal: correct_body p unit (returnM tt) fn (Sreturn None) modifies *)
         eapply correct_body_Sreturn_None.
-        unfold match_res, correct_get_opcode_alu64.match_res.
+        unfold match_res, correct_get_opcode_alu32.match_res.
         intros.
         get_invariant _st.
         unfold stateM_correct in c3.
@@ -734,77 +724,26 @@ Ltac correct_forward L :=
         reflexivity.
       + reflexivity.
       + intros.
-        get_invariant _opcode_alu64.
+        get_invariant _opcode_alu32.
         unfold exec_expr.
         rewrite p0. f_equal.
-        unfold correct_get_opcode_alu64.match_res in c3.
-        unfold opcode_alu64_correct in c3.
-        (* opcode_alu64_correct should be a mapping between opcodes and int *)
+        unfold correct_get_opcode_alu32.match_res in c3.
+        unfold opcode_alu32_correct in c3.
+        (* opcode_alu32_correct should be a mapping between opcodes and int *)
         destruct c3; assumption.
       + compute. intuition congruence.
-    - (**r op_BPF_LSH64 *)
+    - (**r op_BPF_LSH32 *)
       eapply correct_statement_switch with (n:= 96).
       + simpl.
         eapply correct_statement_seq_body_drop.
         intros.
-        eapply correct_statement_seq_body with (modifies1:=nil).
-        change_app_for_statement.
-        eapply correct_statement_call with (has_cast := false).
-        my_reflex.
-        reflexivity.
-        reflexivity.
-        typeclasses eauto.
-        { unfold modifies.
-          unfold var_inv_preserve.
-          unfold match_temp_env.
-          intros.
-          inversion H1; subst; clear H1.
-          inversion H5; subst; clear H5.
-          inversion H6; subst; clear H6.
-          inversion H7; subst; clear H7.
-          inversion H8; subst; clear H8.
-          inversion H9; subst; clear H9.
-          repeat constructor;auto.
-
-          revert H3. (**r moves the hypotheses  to the goal *)
-          unfold match_elt,fst.
-          destruct (Maps.PTree.get _st le1); try congruence.
-          unfold snd.
-          intro HH ; destruct HH ; split; auto.
-          unfold correct_upd_reg.match_res in H0.
-          unfold stateM_correct in *.
-          unfold unmodifies_effect in H.
-          destruct H as (Hm & Hst); subst.
-          tauto.
-        }
-        reflexivity.
-        reflexivity.
-        reflexivity.
-        simpl.
-        Hdisj_false.
-        simpl.
-        Hdisj_false.
-        reflexivity.
-        reflexivity.
-
-        unfold INV; intro H.
-        correct_Forall.
-        get_invariant _src64.
-        unfold val64_correct,stateless in c3.
-        destruct c3 as (Hv_eq & (vl & Hvl_eq)); subst.
-        exists (Vlong vl :: nil).
-        unfold map_opt, exec_expr.
-        rewrite p0.
-        split; [reflexivity |].
-        intros.
-        simpl.
-        unfold stateless,val64_correct.
-        intuition.
-        eexists ; reflexivity.
-        intros.
+        unfold rBPFValues.compu_lt_32.
         (**r correct_body p unit (if rBPFValues.compu_lt_32 ... *)
         eapply correct_statement_if_body_expr.
-        destruct (rBPFValues.compu_lt_32 _ _) eqn: Hlt_64.
+        destruct (match c0 with
+                  | Vint n1 => Int.ltu n1 (Int.repr 32)
+                  | _ => false
+                  end) eqn: Hlt_32.
 
         eapply correct_statement_seq_body_unit.
         change_app_for_statement.
@@ -816,7 +755,6 @@ Ltac correct_forward L :=
         typeclasses eauto.
         unfold correct_upd_reg.match_res. intuition.
         { unfold modifies.
-          instantiate (1:= state_block).
           instantiate (1:= ins_block).
           instantiate (1:= mrs_block).
           unfold var_inv_preserve.
@@ -831,7 +769,7 @@ Ltac correct_forward L :=
           inversion H10; subst; clear H10.
           repeat constructor;auto.
 
-          revert H5. (**r moves the hypotheses  to the goal *)
+          revert H3. (**r moves the hypotheses  to the goal *)
           unfold match_elt,fst.
           destruct (Maps.PTree.get _ _); [| congruence].
           unfold snd.
@@ -850,42 +788,40 @@ Ltac correct_forward L :=
         correct_Forall.
         get_invariant _st.
         get_invariant _dst.
-        get_invariant _dst64.
-        get_invariant _src32.
+        get_invariant _dst32.
+        get_invariant _src32. (*
         unfold stateless, stateM_correct in c3.
         destruct c3 as (Hv_eq & Hst); subst.
-        unfold stateless, reg_correct in c4.
-        unfold stateless, val64_correct in c5.
+        unfold stateless, reg_correct in c4. *)
+        unfold stateless, valu32_correct in c5.
         destruct c5 as (Hv1_eq & (vl & Hvl_eq)); subst.
-        unfold correct_reg64_to_reg32.match_res, valu32_correct in c6.
+        unfold stateless, valu32_correct in c6.
         destruct c6 as (Hv2_eq & (vi & Hvi_eq)); subst.
-        exists ((Vptr state_block Ptrofs.zero) :: (Vint (Int.repr (id_of_reg c1))) :: (Val.shll (Vlong vl) (Vint vi)) :: nil). (**r star here *)
+        exists (v :: v0 :: (Val.longofintu (Val.shl (Vint vl) (Vint vi))) :: nil). (**r star here *)
         unfold map_opt, exec_expr.
         rewrite p0, p1, p2, p3.
-        simpl.
+        unfold Cop.sem_binary_operation, typeof.
         unfold Cop.sem_shl, Cop.sem_shift; simpl.
-        change Int64.iwordsize' with (Int.repr 64).
-        unfold rBPFValues.compu_lt_32 in Hlt_64.
-        rewrite Hlt_64.
-        split.
-        unfold Int64.shl', Int64.shl.
-        rewrite Hint_unsigned_int64; reflexivity.
-        intros.
-        unfold correct_upd_reg.stateM_correct, stateless, reg_correct, val64_correct.
-        simpl.
+        change Int.iwordsize with (Int.repr 32).
+        rewrite Hlt_32.
+        split; [reflexivity | ].
+        intros; simpl.
         intuition.
-        eexists ; reflexivity.
+        unfold stateless,val64_correct.
+        split; [reflexivity | eexists ; reflexivity].
         intros.
 
         (**r goal: correct_body p unit (returnM tt) fn (Sreturn None) modifies *)
         eapply correct_body_Sreturn_None.
-        unfold match_res, correct_get_opcode_alu64.match_res.
+        unfold match_res, correct_get_opcode_alu32.match_res.
         intros.
         get_invariant _st.
         unfold stateM_correct in c3.
         destruct c3 as (_ & c3); assumption.
         reflexivity.
 
+        change (upd_flag Flag.BPF_ILLEGAL_SHIFT) with
+          (bindM (upd_flag Flag.BPF_ILLEGAL_SHIFT) (fun _ : unit => returnM tt)).
         (**r goal: correct_body p unit (upd_flag Flag.BPF_ILLEGAL_SHIFT) fn ... *)
         eapply correct_statement_seq_body_unit.
         change_app_for_statement.
@@ -911,7 +847,7 @@ Ltac correct_forward L :=
           inversion H10; subst; clear H10.
           repeat constructor;auto.
 
-          revert H5. (**r moves the hypotheses  to the goal *)
+          revert H3. (**r moves the hypotheses  to the goal *)
           unfold match_elt,fst.
           destruct (Maps.PTree.get _ _); try congruence.
           unfold snd.
@@ -944,7 +880,7 @@ Ltac correct_forward L :=
 
         (**r goal: correct_body p unit (returnM tt) fn (Sreturn None) modifies *)
         eapply correct_body_Sreturn_None.
-        unfold match_res, correct_get_opcode_alu64.match_res.
+        unfold match_res, correct_get_opcode_alu32.match_res.
         intros.
         get_invariant _st.
         unfold stateM_correct in c3.
@@ -954,86 +890,34 @@ Ltac correct_forward L :=
 
         intros.
         get_invariant _src32.
-        unfold correct_reg64_to_reg32.match_res, valu32_correct in c3.
+        unfold stateless, valu32_correct in c3.
         destruct c3 as (Hv_eq & vi & Hvi_eq); subst.
         unfold exec_expr.
         rewrite p0.
         unfold Cop.sem_binary_operation, Cop.sem_cmp, Cop.sem_binarith, Cop.sem_cast; simpl.
         reflexivity.
-        reflexivity.
 
       + reflexivity.
       + intros.
-        get_invariant _opcode_alu64.
-        unfold correct_get_opcode_alu64.match_res, opcode_alu64_correct in c3.
+        get_invariant _opcode_alu32.
+        unfold correct_get_opcode_alu32.match_res, opcode_alu32_correct in c3.
         unfold exec_expr.
         rewrite p0. f_equal.
-        (* opcode_alu64_correct should be a mapping between opcodes and int *)
+        (* opcode_alu32_correct should be a mapping between opcodes and int *)
         destruct c3; assumption.
       + compute. intuition congruence.
-    - (**r op_BPF_RSH64 *)
+    - (**r op_BPF_RSH32 *)
       eapply correct_statement_switch with (n:= 112).
       + simpl.
         eapply correct_statement_seq_body_drop.
         intros.
-        eapply correct_statement_seq_body with (modifies1:=nil).
-        change_app_for_statement.
-        eapply correct_statement_call with (has_cast := false).
-        my_reflex.
-        reflexivity.
-        reflexivity.
-        typeclasses eauto.
-        { unfold modifies.
-          unfold var_inv_preserve.
-          unfold match_temp_env.
-          intros.
-          inversion H1; subst; clear H1.
-          inversion H5; subst; clear H5.
-          inversion H6; subst; clear H6.
-          inversion H7; subst; clear H7.
-          inversion H8; subst; clear H8.
-          inversion H9; subst; clear H9.
-          repeat constructor;auto.
-
-          revert H3. (**r moves the hypotheses  to the goal *)
-          unfold match_elt,fst.
-          destruct (Maps.PTree.get _ _); try congruence.
-          unfold snd.
-          intro HH ; destruct HH ; split; auto.
-          unfold correct_upd_reg.match_res in H0.
-          unfold stateM_correct in *.
-          unfold unmodifies_effect in H.
-          destruct H as (Hm & Hst); subst.
-          tauto.
-        }
-        reflexivity.
-        reflexivity.
-        reflexivity.
-        simpl.
-        Hdisj_false.
-        simpl.
-        Hdisj_false.
-        reflexivity.
-        reflexivity.
-
-        unfold INV; intro H.
-        correct_Forall.
-        get_invariant _src64.
-        unfold val64_correct,stateless in c3.
-        destruct c3 as (Hv_eq & (vl & Hvl_eq)); subst.
-        exists (Vlong vl :: nil).
-        unfold map_opt, exec_expr.
-        rewrite p0.
-        split; [reflexivity |].
-        intros.
-        simpl.
-        unfold stateless,val64_correct.
-        intuition.
-        eexists ; reflexivity.
-        intros.
+        unfold rBPFValues.compu_lt_32.
         (**r correct_body p unit (if rBPFValues.compu_lt_32 ... *)
         eapply correct_statement_if_body_expr.
-        destruct (rBPFValues.compu_lt_32 _ _) eqn: Hlt_64.
+        destruct (match c0 with
+                  | Vint n1 => Int.ltu n1 (Int.repr 32)
+                  | _ => false
+                  end) eqn: Hlt_32.
 
         eapply correct_statement_seq_body_unit.
         change_app_for_statement.
@@ -1045,7 +929,6 @@ Ltac correct_forward L :=
         typeclasses eauto.
         unfold correct_upd_reg.match_res. intuition.
         { unfold modifies.
-          instantiate (1:= state_block).
           instantiate (1:= ins_block).
           instantiate (1:= mrs_block).
           unfold var_inv_preserve.
@@ -1060,7 +943,7 @@ Ltac correct_forward L :=
           inversion H10; subst; clear H10.
           repeat constructor;auto.
 
-          revert H5. (**r moves the hypotheses  to the goal *)
+          revert H3. (**r moves the hypotheses  to the goal *)
           unfold match_elt,fst.
           destruct (Maps.PTree.get _ _); [| congruence].
           unfold snd.
@@ -1079,42 +962,39 @@ Ltac correct_forward L :=
         correct_Forall.
         get_invariant _st.
         get_invariant _dst.
-        get_invariant _dst64.
+        get_invariant _dst32.
         get_invariant _src32.
-        unfold stateless, stateM_correct in c3.
-        destruct c3 as (Hv_eq & Hst); subst.
-        unfold stateless, reg_correct in c4.
-        unfold stateless, val64_correct in c5.
+        unfold stateless, valu32_correct in c5.
         destruct c5 as (Hv1_eq & (vl & Hvl_eq)); subst.
-        unfold correct_reg64_to_reg32.match_res, valu32_correct in c6.
+        unfold stateless, valu32_correct in c6.
         destruct c6 as (Hv2_eq & (vi & Hvi_eq)); subst.
-        exists ((Vptr state_block Ptrofs.zero) :: (Vint (Int.repr (id_of_reg c1))) :: (Val.shrlu (Vlong vl) (Vint vi)) :: nil). (**r star here *)
+        exists (v :: v0 :: (Val.longofintu (Val.shru (Vint vl) (Vint vi))) :: nil). (**r star here *)
         unfold map_opt, exec_expr.
         rewrite p0, p1, p2, p3.
-        simpl.
+        unfold Cop.sem_binary_operation, typeof.
         unfold Cop.sem_shr, Cop.sem_shift; simpl.
-        change Int64.iwordsize' with (Int.repr 64).
-        unfold rBPFValues.compu_lt_32 in Hlt_64.
-        rewrite Hlt_64.
-        split.
-        unfold Int64.shru', Int64.shru.
-        rewrite Hint_unsigned_int64; reflexivity.
-        intros.
-        unfold correct_upd_reg.stateM_correct, stateless, reg_correct, val64_correct.
-        simpl.
+        change Int.iwordsize with (Int.repr 32).
+        rewrite Hlt_32.
+        unfold Cop.sem_cast; simpl.
+        split; [reflexivity | ].
+        intros; simpl.
         intuition.
-        eexists ; reflexivity.
+        unfold stateless,val64_correct.
+        split; [reflexivity | eexists ; reflexivity].
         intros.
+
 
         (**r goal: correct_body p unit (returnM tt) fn (Sreturn None) modifies *)
         eapply correct_body_Sreturn_None.
-        unfold match_res, correct_get_opcode_alu64.match_res.
+        unfold match_res, correct_get_opcode_alu32.match_res.
         intros.
         get_invariant _st.
         unfold stateM_correct in c3.
         destruct c3 as (_ & c3); assumption.
         reflexivity.
 
+        change (upd_flag Flag.BPF_ILLEGAL_SHIFT) with
+          (bindM (upd_flag Flag.BPF_ILLEGAL_SHIFT) (fun _ : unit => returnM tt)).
         (**r goal: correct_body p unit (upd_flag Flag.BPF_ILLEGAL_SHIFT) fn ... *)
         eapply correct_statement_seq_body_unit.
         change_app_for_statement.
@@ -1140,7 +1020,7 @@ Ltac correct_forward L :=
           inversion H10; subst; clear H10.
           repeat constructor;auto.
 
-          revert H5. (**r moves the hypotheses  to the goal *)
+          revert H3. (**r moves the hypotheses  to the goal *)
           unfold match_elt,fst.
           destruct (Maps.PTree.get _ _); try congruence.
           unfold snd.
@@ -1173,7 +1053,7 @@ Ltac correct_forward L :=
 
         (**r goal: correct_body p unit (returnM tt) fn (Sreturn None) modifies *)
         eapply correct_body_Sreturn_None.
-        unfold match_res, correct_get_opcode_alu64.match_res.
+        unfold match_res, correct_get_opcode_alu32.match_res.
         intros.
         get_invariant _st.
         unfold stateM_correct in c3.
@@ -1189,15 +1069,14 @@ Ltac correct_forward L :=
         rewrite p0.
         unfold Cop.sem_binary_operation, Cop.sem_cmp, Cop.sem_binarith, Cop.sem_cast; simpl.
         reflexivity.
-        reflexivity.
 
       + reflexivity.
       + intros.
-        get_invariant _opcode_alu64.
-        unfold correct_get_opcode_alu64.match_res, opcode_alu64_correct in c3.
+        get_invariant _opcode_alu32.
+        unfold correct_get_opcode_alu32.match_res, opcode_alu32_correct in c3.
         unfold exec_expr.
         rewrite p0. f_equal.
-        (* opcode_alu64_correct should be a mapping between opcodes and int *)
+        (* opcode_alu32_correct should be a mapping between opcodes and int *)
         destruct c3; assumption.
       + compute. intuition congruence.
     - (**r op_BPF_NEG64 *)
@@ -1208,7 +1087,7 @@ Ltac correct_forward L :=
         intros.
         (**r because upd_reg return unit, here we use *_unit? *)
         eapply correct_statement_if_body_expr.
-        destruct (c2 =? 135)%nat eqn: Hneg_eq.
+        destruct (c2 =? 132)%nat eqn: Hneg_eq.
 
 
         eapply correct_statement_seq_body_unit.
@@ -1222,10 +1101,10 @@ Ltac correct_forward L :=
         unfold correct_upd_reg.match_res. intuition.
         { unfold modifies.
           instantiate (1:= ins_block).
+          instantiate (1:= mrs_block).
           unfold var_inv_preserve.
           unfold match_temp_env.
           intros.
-          instantiate (1 := mrs_block) in H0.
           inversion H1; subst; clear H1.
           inversion H5; subst; clear H5.
           inversion H6; subst; clear H6.
@@ -1253,33 +1132,34 @@ Ltac correct_forward L :=
         correct_Forall.
         get_invariant _st.
         get_invariant _dst.
-        get_invariant _dst64.
-        get_invariant _src64.
-        unfold val64_correct,stateless in c5, c6.
+        get_invariant _dst32.
+        get_invariant _src32.
+        unfold valu32_correct,stateless in c5, c6.
         destruct c5 as (Hv1_eq & (vl1 & Hvl1_eq)); subst.
         destruct c6 as (Hv2_eq & (vl2 & Hvl2_eq)); subst.
-        exists (v :: v0 :: Vlong (Int64.neg vl1) :: nil). (**r star here *)
+        exists (v :: v0 :: Val.longofintu (Val.neg (Vint vl1)) :: nil). (**r star here *)
         unfold map_opt, exec_expr.
-        rewrite p0.
-        rewrite p1. rewrite p2.
-        split.
-        unfold Cop.sem_unary_operation; simpl.
-        reflexivity.
-        intros.
-        simpl.
+        rewrite p0, p1, p2.
+        unfold Cop.sem_unary_operation, typeof.
+        unfold Cop.sem_neg; simpl.
+        split; [reflexivity | ].
+        intros; simpl.
         intuition.
         unfold stateless,val64_correct.
-        split; auto. eexists ; reflexivity.
+        split; [reflexivity | eexists ; reflexivity].
         intros.
 
         (**r goal: correct_body p unit (returnM tt) fn (Sreturn None) modifies *)
         eapply correct_body_Sreturn_None.
-        unfold match_res, correct_get_opcode_alu64.match_res.
+        unfold match_res, correct_get_opcode_alu32.match_res.
         intros.
         get_invariant _st.
         unfold stateM_correct in c3.
         destruct c3 as (_ & c3); assumption.
         reflexivity.
+
+        change (upd_flag Flag.BPF_ILLEGAL_INSTRUCTION) with
+          (bindM (upd_flag Flag.BPF_ILLEGAL_INSTRUCTION) (fun _ : unit => returnM tt)).
         eapply correct_statement_seq_body_unit.
         change_app_for_statement.
         (**r goal: correct_statement p unit (app f a) fn (Scall None (Evar ... *)
@@ -1291,10 +1171,10 @@ Ltac correct_forward L :=
         unfold correct_upd_flag.match_res. intuition.
         { unfold modifies.
           instantiate (1:= ins_block).
+          instantiate (1 := mrs_block).
           unfold var_inv_preserve.
           unfold match_temp_env.
           intros.
-          instantiate (1 := mrs_block) in H0.
           inversion H1; subst; clear H1.
           inversion H5; subst; clear H5.
           inversion H6; subst; clear H6.
@@ -1322,9 +1202,9 @@ Ltac correct_forward L :=
         correct_Forall.
         get_invariant _st.
         get_invariant _dst.
-        get_invariant _dst64.
-        get_invariant _src64.
-        unfold val64_correct,stateless in c5, c6.
+        get_invariant _dst32.
+        get_invariant _src32.
+        unfold valu32_correct,stateless in c5, c6.
         destruct c5 as (Hv1_eq & (vl1 & Hvl1_eq)); subst.
         destruct c6 as (Hv2_eq & (vl2 & Hvl2_eq)); subst.
         exists (v ::Vint (Int.neg (Int.repr 1)) :: nil). (**r star here: it should be -1 *)
@@ -1336,13 +1216,13 @@ Ltac correct_forward L :=
         intros.
         simpl.
         intuition.
-        unfold stateless,val64_correct.
+        unfold stateless,valu32_correct.
         split; auto.
         intros.
 
         (**r goal: correct_body p unit (returnM tt) fn (Sreturn None) modifies *)
         eapply correct_body_Sreturn_None.
-        unfold match_res, correct_get_opcode_alu64.match_res.
+        unfold match_res, correct_get_opcode_alu32.match_res.
         intros.
         get_invariant _st.
         unfold stateM_correct in c3.
@@ -1357,7 +1237,7 @@ Ltac correct_forward L :=
         unfold stateless, opcode_correct in c3.
         destruct c3 as (Hv_eq & Hrange).
         rewrite <- Hv_eq.
-        destruct (c2 =? 135)%nat eqn: Hc2_eq.
+        destruct (c2 =? 132)%nat eqn: Hc2_eq.
         rewrite Nat.eqb_eq in Hc2_eq.
         subst.
         simpl.
@@ -1366,7 +1246,7 @@ Ltac correct_forward L :=
         rewrite Nat.eqb_neq in Hc2_eq.
         simpl.
         unfold Cop.sem_cmp, Cop.sem_binarith; simpl.
-        assert (Hneq: Int.eq (Int.repr (Z.of_nat c2)) (Int.repr 135) = false). {
+        assert (Hneq: Int.eq (Int.repr (Z.of_nat c2)) (Int.repr 132) = false). {
           apply Int.eq_false.
           apply nat8_neq_k; auto; lia.
         }
@@ -1375,23 +1255,24 @@ Ltac correct_forward L :=
 
       + reflexivity.
       + intros.
-        get_invariant _opcode_alu64.
+        get_invariant _opcode_alu32.
         unfold exec_expr.
         rewrite p0. f_equal.
-        unfold correct_get_opcode_alu64.match_res in c3.
-        unfold opcode_alu64_correct in c3.
-        change (Int.repr (Z.of_nat (Nat.land 135 240))) with (Int.repr 128) in c3.
+        unfold correct_get_opcode_alu32.match_res in c3.
+        unfold opcode_alu32_correct in c3.
+        change (Int.repr (Z.of_nat (Nat.land 132 240))) with (Int.repr 128) in c3.
         assumption.
       + compute. intuition congruence.
-    - (**r op_BPF_MOD64 *)
+    - (**r op_BPF_MOD32 *)
       eapply correct_statement_switch with (n:= 144).
       + simpl.
         (**r s1 -> (Ssequence s1 s2) *)
         eapply correct_statement_seq_body_drop.
         intros.
-        (**r correct_body p unit (if rBPFValues.compl_ne c0 val64_zero then ... *)
+        unfold Vzero.
+        (**r correct_body p unit (if rBPFValues.compl_ne c0 valu32_zero then ... *)
         eapply correct_statement_if_body_expr.
-        destruct (rBPFValues.compl_ne c0 (Vlong Int64.zero)) eqn: Hmod_zero.
+        destruct (rBPFValues.comp_ne_32 c0 (Vint Int.zero)) eqn: Hmod_zero.
 
 
         eapply correct_statement_seq_body_unit.
@@ -1405,10 +1286,10 @@ Ltac correct_forward L :=
         unfold correct_upd_reg.match_res. intuition.
         { unfold modifies.
           instantiate (1:= ins_block).
+          instantiate (1 := mrs_block).
           unfold var_inv_preserve.
           unfold match_temp_env.
           intros.
-          instantiate (1 := mrs_block) in H0.
           inversion H1; subst; clear H1.
           inversion H5; subst; clear H5.
           inversion H6; subst; clear H6.
@@ -1436,44 +1317,41 @@ Ltac correct_forward L :=
         correct_Forall.
         get_invariant _st.
         get_invariant _dst.
-        get_invariant _dst64.
-        get_invariant _src64.
-        unfold val64_correct,stateless in c5, c6.
+        get_invariant _dst32.
+        get_invariant _src32.
+        unfold valu32_correct,stateless in c5, c6.
         destruct c5 as (Hv1_eq & (vl1 & Hvl1_eq)); subst.
         destruct c6 as (Hv2_eq & (vl2 & Hvl2_eq)); subst.
-        unfold rBPFValues.val64_modlu, Val.modlu. (**r star here *)
-        unfold rBPFValues.compl_ne, val64_zero in Hmod_zero.
+        unfold rBPFValues.val32_modu, Val.modu. (**r star here *)
+        unfold rBPFValues.comp_ne_32 in Hmod_zero.
         rewrite Bool.negb_true_iff in Hmod_zero.
         rewrite Hmod_zero.
-        exists (v ::v0 :: Vlong (Int64.modu vl1 vl2) :: nil). (**r star here *)
+        exists (v ::v0 :: Val.longofintu (Vint (Int.modu vl1 vl2)) :: nil). (**r star here *)
         unfold map_opt, exec_expr.
-        rewrite p0.
-        rewrite p1. rewrite p2. rewrite p3.
-        split.
-        simpl.
-        unfold Cop.sem_mod, Cop.sem_binarith;
-        simpl.
-        Transparent Archi.ptr64.
-        unfold Cop.sem_cast; simpl.
+        rewrite p0, p1, p2, p3.
+        unfold Cop.sem_binary_operation, typeof.
+        unfold Cop.sem_mod, Cop.sem_binarith; simpl.
         rewrite Hmod_zero.
-        reflexivity.
-        intros.
-        simpl.
+        unfold Cop.sem_cast; simpl.
+        split; [reflexivity | ].
+        intros; simpl.
         intuition.
-        unfold stateless,val64_correct.
-        split; auto. eexists ; reflexivity.
+        unfold stateless, val64_correct.
+        split; [reflexivity | eexists ; reflexivity].
         intros.
 
         (**r goal: correct_body p unit (returnM tt) fn (Sreturn None) modifies *)
         eapply correct_body_Sreturn_None.
-        unfold match_res, correct_get_opcode_alu64.match_res.
+        unfold match_res, correct_get_opcode_alu32.match_res.
         intros.
         get_invariant _st.
         unfold stateM_correct in c3.
         destruct c3 as (_ & c3); assumption.
         reflexivity.
 
-        unfold rBPFValues.compl_ne, val64_zero in Hmod_zero.
+        change (upd_flag Flag.BPF_ILLEGAL_DIV) with
+          (bindM (upd_flag Flag.BPF_ILLEGAL_DIV) (fun _ : unit => returnM tt)).
+        unfold rBPFValues.comp_ne_32 in Hmod_zero.
         (**r goal: correct_body p unit (upd_flag Flag.BPF_ILLEGAL_DIV) fn ... *)
         eapply correct_statement_seq_body_unit.
         change_app_for_statement.
@@ -1486,10 +1364,10 @@ Ltac correct_forward L :=
         unfold correct_upd_flag.match_res. intuition.
         { unfold modifies.
           instantiate (1:= ins_block).
+          instantiate (1 := mrs_block).
           unfold var_inv_preserve.
           unfold match_temp_env.
           intros.
-          instantiate (1 := mrs_block) in H0.
           inversion H1; subst; clear H1.
           inversion H5; subst; clear H5.
           inversion H6; subst; clear H6.
@@ -1517,9 +1395,9 @@ Ltac correct_forward L :=
         correct_Forall.
         get_invariant _st.
         get_invariant _dst.
-        get_invariant _dst64.
-        get_invariant _src64.
-        unfold val64_correct,stateless in c5, c6.
+        get_invariant _dst32.
+        get_invariant _src32.
+        unfold valu32_correct,stateless in c5, c6.
         destruct c5 as (Hv1_eq & (vl1 & Hvl1_eq)); subst.
         destruct c6 as (Hv2_eq & (vl2 & Hvl2_eq)); subst.
         exists (v ::Vint (Int.neg (Int.repr 9)) :: nil). (**r star here *)
@@ -1531,13 +1409,13 @@ Ltac correct_forward L :=
         intros.
         simpl.
         intuition.
-        unfold stateless,val64_correct.
+        unfold stateless,valu32_correct.
         split; auto.
         intros.
 
         (**r goal: correct_body p unit (returnM tt) fn (Sreturn None) modifies *)
         eapply correct_body_Sreturn_None.
-        unfold match_res, correct_get_opcode_alu64.match_res.
+        unfold match_res, correct_get_opcode_alu32.match_res.
         intros.
         get_invariant _st.
         unfold stateM_correct in c3.
@@ -1546,26 +1424,26 @@ Ltac correct_forward L :=
         reflexivity.
 
         intros.
-        get_invariant _src64.
+        get_invariant _src32.
         unfold exec_expr.
-        rewrite p0. unfold val64_zero, rBPFValues.compl_ne, Int64.zero.
+        rewrite p0. unfold rBPFValues.comp_ne_32, Int.zero.
         unfold Cop.sem_binary_operation, Cop.sem_cmp, Cop.sem_binarith, Cop.sem_cast; simpl.
-        unfold stateless, val64_correct in c3.
+        unfold stateless, valu32_correct in c3.
         destruct c3 as (c3_0 & c3_vl & c3_1).
         subst.
         reflexivity.
 
       + reflexivity.
       + intros.
-        get_invariant _opcode_alu64.
+        get_invariant _opcode_alu32.
         unfold exec_expr.
         rewrite p0. f_equal.
-        unfold correct_get_opcode_alu64.match_res in c3.
-        unfold opcode_alu64_correct in c3.
-        (* opcode_alu64_correct should be a mapping between opcodes and int *)
+        unfold correct_get_opcode_alu32.match_res in c3.
+        unfold opcode_alu32_correct in c3.
+        (* opcode_alu32_correct should be a mapping between opcodes and int *)
         destruct c3; assumption.
       + compute. intuition congruence.
-    - (**r op_BPF_XOR64 *)
+    - (**r op_BPF_XOR32 *)
       eapply correct_statement_switch with (n:= 160).
       + simpl.
         (**r s1 -> (Ssequence s1 s2) *)
@@ -1583,10 +1461,10 @@ Ltac correct_forward L :=
         unfold correct_upd_reg.match_res. intuition.
         { unfold modifies.
           instantiate (1:= ins_block).
+          instantiate (1 := mrs_block).
           unfold var_inv_preserve.
           unfold match_temp_env.
           intros.
-          instantiate (1 := mrs_block) in H0.
           inversion H1; subst; clear H1.
           inversion H5; subst; clear H5.
           inversion H6; subst; clear H6.
@@ -1614,27 +1492,28 @@ Ltac correct_forward L :=
         correct_Forall.
         get_invariant _st.
         get_invariant _dst.
-        get_invariant _dst64.
-        get_invariant _src64.
-        unfold val64_correct,stateless in c5, c6.
+        get_invariant _dst32.
+        get_invariant _src32.
+        unfold valu32_correct,stateless in c5, c6.
         destruct c5 as (Hv1_eq & (vl1 & Hvl1_eq)); subst.
         destruct c6 as (Hv2_eq & (vl2 & Hvl2_eq)); subst.
-        exists (v ::v0 :: Vlong (Int64.xor vl1 vl2) :: nil). (**r star here *)
+
+        exists (v ::v0 :: Val.longofintu (Vint (Int.xor vl1 vl2)) :: nil). (**r star here *)
         unfold map_opt, exec_expr.
-        rewrite p0.
-        rewrite p1. rewrite p2. rewrite p3.
-        split.
-        reflexivity.
-        intros.
-        simpl.
+        rewrite p0, p1, p2, p3.
+        unfold Cop.sem_binary_operation, typeof.
+        unfold Cop.sem_xor, Cop.sem_binarith; simpl.
+        split; [reflexivity | ].
+        intros; simpl.
         intuition.
-        unfold stateless,val64_correct.
-        split; auto. eexists ; reflexivity.
+        unfold stateless, val64_correct.
+        split; [reflexivity | eexists ; reflexivity].
         intros.
+
 
         (**r goal: correct_body p unit (returnM tt) fn (Sreturn None) modifies *)
         eapply correct_body_Sreturn_None.
-        unfold match_res, correct_get_opcode_alu64.match_res.
+        unfold match_res, correct_get_opcode_alu32.match_res.
         intros.
         get_invariant _st.
         unfold stateM_correct in c3.
@@ -1642,15 +1521,15 @@ Ltac correct_forward L :=
         reflexivity.
       + reflexivity.
       + intros.
-        get_invariant _opcode_alu64.
+        get_invariant _opcode_alu32.
         unfold exec_expr.
         rewrite p0. f_equal.
-        unfold correct_get_opcode_alu64.match_res in c3.
-        unfold opcode_alu64_correct in c3.
-        (* opcode_alu64_correct should be a mapping between opcodes and int *)
+        unfold correct_get_opcode_alu32.match_res in c3.
+        unfold opcode_alu32_correct in c3.
+        (* opcode_alu32_correct should be a mapping between opcodes and int *)
         destruct c3; assumption.
       + compute. intuition congruence.
-    - (**r op_BPF_MOV64 *)
+    - (**r op_BPF_MOV32 *)
       eapply correct_statement_switch with (n:= 176).
       + simpl.
         (**r s1 -> (Ssequence s1 s2) *)
@@ -1668,10 +1547,10 @@ Ltac correct_forward L :=
         unfold correct_upd_reg.match_res. intuition.
         { unfold modifies.
           instantiate (1:= ins_block).
+          instantiate (1 := mrs_block).
           unfold var_inv_preserve.
           unfold match_temp_env.
           intros.
-          instantiate (1 := mrs_block) in H0.
           inversion H1; subst; clear H1.
           inversion H5; subst; clear H5.
           inversion H6; subst; clear H6.
@@ -1699,27 +1578,25 @@ Ltac correct_forward L :=
         correct_Forall.
         get_invariant _st.
         get_invariant _dst.
-        get_invariant _dst64.
-        get_invariant _src64.
-        unfold val64_correct,stateless in c5, c6.
+        get_invariant _dst32.
+        get_invariant _src32.
+        unfold valu32_correct,stateless in c5, c6.
         destruct c5 as (Hv1_eq & (vl1 & Hvl1_eq)); subst.
         destruct c6 as (Hv2_eq & (vl2 & Hvl2_eq)); subst.
-        exists (v ::v0 :: Vlong (vl2) :: nil). (**r star here *)
+        exists (v ::v0 :: (Val.longofintu (Vint vl2)) :: nil). (**r star here *)
         unfold map_opt, exec_expr.
-        rewrite p0.
-        rewrite p1. rewrite p3.
-        split.
-        reflexivity.
-        intros.
-        simpl.
+        rewrite p0, p1, p3.
+        unfold Cop.sem_cast, typeof, Cop.classify_cast; simpl.
+        split; [reflexivity | ].
+        intros; simpl.
         intuition.
         unfold stateless,val64_correct.
-        split; auto. eexists ; reflexivity.
+        split; [reflexivity | eexists ; reflexivity].
         intros.
 
         (**r goal: correct_body p unit (returnM tt) fn (Sreturn None) modifies *)
         eapply correct_body_Sreturn_None.
-        unfold match_res, correct_get_opcode_alu64.match_res.
+        unfold match_res, correct_get_opcode_alu32.match_res.
         intros.
         get_invariant _st.
         unfold stateM_correct in c3.
@@ -1727,79 +1604,28 @@ Ltac correct_forward L :=
         reflexivity.
       + reflexivity.
       + intros.
-        get_invariant _opcode_alu64.
+        get_invariant _opcode_alu32.
         unfold exec_expr.
         rewrite p0. f_equal.
-        unfold correct_get_opcode_alu64.match_res in c3.
-        unfold opcode_alu64_correct in c3.
-        (* opcode_alu64_correct should be a mapping between opcodes and int *)
-        change (Int.repr (Z.of_nat (Nat.land 183 240))) with (Int.repr 176) in c3.
-        change (Int.repr (Z.of_nat (Nat.land 191 240))) with (Int.repr 176) in c3.
+        unfold correct_get_opcode_alu32.match_res in c3.
+        unfold opcode_alu32_correct in c3.
+        (* opcode_alu32_correct should be a mapping between opcodes and int *)
+        change (Int.repr (Z.of_nat (Nat.land 180 240))) with (Int.repr 176) in c3.
+        change (Int.repr (Z.of_nat (Nat.land 188 240))) with (Int.repr 176) in c3.
         destruct c3; assumption.
       + compute. intuition congruence.
-    - (**r op_BPF_ARSH64 *)
+    - (**r op_BPF_ARSH32 *)
       eapply correct_statement_switch with (n:= 192).
       + simpl.
         eapply correct_statement_seq_body_drop.
         intros.
-        eapply correct_statement_seq_body with (modifies1:=nil).
-        change_app_for_statement.
-        eapply correct_statement_call with (has_cast := false).
-        my_reflex.
-        reflexivity.
-        reflexivity.
-        typeclasses eauto.
-        { unfold modifies.
-          unfold var_inv_preserve.
-          unfold match_temp_env.
-          intros.
-          inversion H1; subst; clear H1.
-          inversion H5; subst; clear H5.
-          inversion H6; subst; clear H6.
-          inversion H7; subst; clear H7.
-          inversion H8; subst; clear H8.
-          inversion H9; subst; clear H9.
-          repeat constructor;auto.
-
-          revert H3. (**r moves the hypotheses  to the goal *)
-          unfold match_elt,fst.
-          destruct (Maps.PTree.get _ _); try congruence.
-          unfold snd.
-          intro HH ; destruct HH ; split; auto.
-          unfold correct_upd_reg.match_res in H0.
-          unfold stateM_correct in *.
-          unfold unmodifies_effect in H.
-          destruct H as (Hm & Hst); subst.
-          tauto.
-        }
-        reflexivity.
-        reflexivity.
-        reflexivity.
-        simpl.
-        Hdisj_false.
-        simpl.
-        Hdisj_false.
-        reflexivity.
-        reflexivity.
-
-        unfold INV; intro H.
-        correct_Forall.
-        get_invariant _src64.
-        unfold val64_correct,stateless in c3.
-        destruct c3 as (Hv_eq & (vl & Hvl_eq)); subst.
-        exists (Vlong vl :: nil).
-        unfold map_opt, exec_expr.
-        rewrite p0.
-        split; [reflexivity |].
-        intros.
-        simpl.
-        unfold stateless,val64_correct.
-        intuition.
-        eexists ; reflexivity.
-        intros.
+        unfold rBPFValues.compu_lt_32.
         (**r correct_body p unit (if rBPFValues.compu_lt_32 ... *)
         eapply correct_statement_if_body_expr.
-        destruct (rBPFValues.compu_lt_32 _ _) eqn: Hlt_64.
+        destruct (match c0 with
+                  | Vint n1 => Int.ltu n1 (Int.repr 32)
+                  | _ => false
+                  end) eqn: Hlt_32.
 
         eapply correct_statement_seq_body_unit.
         change_app_for_statement.
@@ -1811,7 +1637,6 @@ Ltac correct_forward L :=
         typeclasses eauto.
         unfold correct_upd_reg.match_res. intuition.
         { unfold modifies.
-          instantiate (1:= state_block).
           instantiate (1:= ins_block).
           instantiate (1:= mrs_block).
           unfold var_inv_preserve.
@@ -1826,7 +1651,7 @@ Ltac correct_forward L :=
           inversion H10; subst; clear H10.
           repeat constructor;auto.
 
-          revert H5. (**r moves the hypotheses  to the goal *)
+          revert H3. (**r moves the hypotheses  to the goal *)
           unfold match_elt,fst.
           destruct (Maps.PTree.get _ _); [| congruence].
           unfold snd.
@@ -1838,50 +1663,52 @@ Ltac correct_forward L :=
         reflexivity.
         reflexivity.
         reflexivity.
-        reflexivity.
+        admit.
         reflexivity.
 
         unfold INV; intro H.
         correct_Forall.
         get_invariant _st.
         get_invariant _dst.
-        get_invariant _dst64.
-        get_invariant _src32.
+        get_invariant _dst32.
+        get_invariant _src32. (*
         unfold stateless, stateM_correct in c3.
         destruct c3 as (Hv_eq & Hst); subst.
-        unfold stateless, reg_correct in c4.
-        unfold stateless, val64_correct in c5.
-        destruct c5 as (Hv1_eq & (vl & Hvl_eq)); subst.
+        unfold stateless, reg_correct in c4. *)
+        unfold stateless, valu32_correct in c5.
+        destruct c5 as (Hv1_eq & (vl & Hvl_eq)).
         unfold correct_reg64_to_reg32.match_res, valu32_correct in c6.
         destruct c6 as (Hv2_eq & (vi & Hvi_eq)); subst.
-        exists ((Vptr state_block Ptrofs.zero) :: (Vint (Int.repr (id_of_reg c1))) :: (Val.shrl (Vlong vl) (Vint vi)) :: nil). (**r star here *)
+        exists (v ::v0 :: (Val.longofint (Val.shr (Vint vl) (Vint vi))) :: nil). (**r star here *)
         unfold map_opt, exec_expr.
         rewrite p0, p1, p2, p3.
         simpl.
         unfold Cop.sem_shr, Cop.sem_shift; simpl.
-        change Int64.iwordsize' with (Int.repr 64).
-        unfold rBPFValues.compu_lt_32 in Hlt_64.
-        rewrite Hlt_64.
+        change Int.iwordsize with (Int.repr 32).
+        rewrite Hlt_32.
         unfold Cop.sem_cast; simpl.
         split.
-        unfold Int64.shr', Int64.shr.
-        rewrite Hint_unsigned_int64; reflexivity.
+        reflexivity.
         intros.
         unfold correct_upd_reg.stateM_correct, stateless, reg_correct, val64_correct.
+        unfold stateM_correct in c3.
         simpl.
         intuition.
         eexists ; reflexivity.
         intros.
 
+
         (**r goal: correct_body p unit (returnM tt) fn (Sreturn None) modifies *)
         eapply correct_body_Sreturn_None.
-        unfold match_res, correct_get_opcode_alu64.match_res.
+        unfold match_res, correct_get_opcode_alu32.match_res.
         intros.
         get_invariant _st.
         unfold stateM_correct in c3.
         destruct c3 as (_ & c3); assumption.
         reflexivity.
 
+        change (upd_flag Flag.BPF_ILLEGAL_SHIFT) with
+          (bindM (upd_flag Flag.BPF_ILLEGAL_SHIFT) (fun _ : unit => returnM tt)).
         (**r goal: correct_body p unit (upd_flag Flag.BPF_ILLEGAL_SHIFT) fn ... *)
         eapply correct_statement_seq_body_unit.
         change_app_for_statement.
@@ -1907,7 +1734,7 @@ Ltac correct_forward L :=
           inversion H10; subst; clear H10.
           repeat constructor;auto.
 
-          revert H5. (**r moves the hypotheses  to the goal *)
+          revert H3. (**r moves the hypotheses  to the goal *)
           unfold match_elt,fst.
           destruct (Maps.PTree.get _ _); try congruence.
           unfold snd.
@@ -1940,7 +1767,7 @@ Ltac correct_forward L :=
 
         (**r goal: correct_body p unit (returnM tt) fn (Sreturn None) modifies *)
         eapply correct_body_Sreturn_None.
-        unfold match_res, correct_get_opcode_alu64.match_res.
+        unfold match_res, correct_get_opcode_alu32.match_res.
         intros.
         get_invariant _st.
         unfold stateM_correct in c3.
@@ -1956,15 +1783,14 @@ Ltac correct_forward L :=
         rewrite p0.
         unfold Cop.sem_binary_operation, Cop.sem_cmp, Cop.sem_binarith, Cop.sem_cast; simpl.
         reflexivity.
-        reflexivity.
 
       + reflexivity.
       + intros.
-        get_invariant _opcode_alu64.
-        unfold correct_get_opcode_alu64.match_res, opcode_alu64_correct in c3.
+        get_invariant _opcode_alu32.
+        unfold correct_get_opcode_alu32.match_res, opcode_alu32_correct in c3.
         unfold exec_expr.
         rewrite p0. f_equal.
-        (* opcode_alu64_correct should be a mapping between opcodes and int *)
+        (* opcode_alu32_correct should be a mapping between opcodes and int *)
         destruct c3; assumption.
       + compute. intuition congruence.
     - (**r op_BPF_ALU64_ILLEGAL_INS *)
@@ -1972,18 +1798,18 @@ Ltac correct_forward L :=
       + reflexivity.
       + intros.
         assert (Hillegal_ins: exists n i,
-          correct_get_opcode_alu64.match_res op_BPF_ALU64_ILLEGAL_INS n st0 m0 /\
+          correct_get_opcode_alu32.match_res op_BPF_ALU32_ILLEGAL_INS n st0 m0 /\
           n = Vint (Int.repr (Z.of_nat (Nat.land i 240))) /\
-          is_illegal_alu64_ins i /\
+          is_illegal_alu32_ins i /\
           exec_expr (Smallstep.globalenv (semantics2 p)) empty_env le0 m0
-            (Etempvar _opcode_alu64 Clightdefs.tuchar) =
+            (Etempvar _opcode_alu32 Clightdefs.tuchar) =
               Some (Vint (Int.repr (Z.of_nat (Nat.land i 240))))).
         {
-          get_invariant _opcode_alu64.
-          unfold correct_get_opcode_alu64.match_res in c3.
+          get_invariant _opcode_alu32.
+          unfold correct_get_opcode_alu32.match_res in c3.
           exists v.
           assert (c3':=c3).
-          unfold opcode_alu64_correct in c3'.
+          unfold opcode_alu32_correct in c3'.
           destruct c3' as (i & V & ILL).
           exists i.
           split ; auto.
@@ -2005,7 +1831,7 @@ Ltac correct_forward L :=
 
         unfold select_switch.
         unfold select_switch_case.
-        unfold is_illegal_alu64_ins in Hill.
+        unfold is_illegal_alu32_ins in Hill.
         repeat match goal with
         | |- context[Coqlib.zeq ?x (Z.of_nat (Nat.land i 240))] =>
             destruct (Coqlib.zeq x (Z.of_nat (Nat.land i 240))) ; try lia
@@ -2015,6 +1841,9 @@ Ltac correct_forward L :=
         (**r s1 -> (Ssequence s1 s2) *)
         eapply correct_statement_seq_body_drop.
         intros.
+
+        change (upd_flag Flag.BPF_ILLEGAL_INSTRUCTION) with
+          (bindM (upd_flag Flag.BPF_ILLEGAL_INSTRUCTION) (fun _ : unit => returnM tt)).
         eapply correct_statement_seq_body_unit.
         change_app_for_statement.
         (**r goal: correct_statement p unit (app f a) fn (Scall None (Evar ... *)
@@ -2026,10 +1855,10 @@ Ltac correct_forward L :=
         unfold correct_upd_flag.match_res. tauto.
         { unfold modifies.
           instantiate (1:= ins_block).
+          instantiate (1 := mrs_block).
           unfold var_inv_preserve.
           unfold match_temp_env.
           intros.
-          instantiate (1 := mrs_block) in H1.
           inversion H2; subst; clear H2.
           inversion H6; subst; clear H6.
           inversion H7; subst; clear H7.
@@ -2072,16 +1901,16 @@ Ltac correct_forward L :=
 
         (**r goal: correct_body p unit (returnM tt) fn (Sreturn None) modifies *)
         eapply correct_body_Sreturn_None.
-        unfold match_res, correct_get_opcode_alu64.match_res.
+        unfold match_res, correct_get_opcode_alu32.match_res.
         intros.
         get_invariant _st.
         unfold stateM_correct in c3.
         destruct c3 as (_ & c3); assumption.
         reflexivity.
-Qed.
+Admitted.
 
-End Step_opcode_alu64.
+End Step_opcode_alu32.
 
 Close Scope Z_scope.
 
-Existing Instance correct_function3_step_opcode_alu64.
+Existing Instance correct_function3_step_opcode_alu32.
