proof/CommonLemmaNat.v
@@ -301,130 +301,6 @@ Proof.
   unfold Nat.land in H. Search Nat.bitwise.
 Qed. *)
 
-Lemma Heven_spec:
-  forall n, Nat.even n = true -> exists m, n = 2*m.
-Proof.
-  intros.
-  rewrite Nat.even_spec in H.
-  rewrite <- Even.even_equiv in H.
-  apply Div2.even_2n in H.
-  destruct H as (p & Hdouble).
-  rewrite Nat.double_twice in Hdouble.
-  exists p; assumption.
-Qed.
-
-Lemma Hodd_spec :
-  forall n, Nat.odd n = true -> exists m, n = 2*m+1.
-Proof.
-  intros.
-  rewrite Nat.odd_spec in H.
-  rewrite <- Even.odd_equiv in H.
-  apply Div2.odd_S2n in H.
-  destruct H as (p & Hdouble).
-  rewrite Nat.double_twice in Hdouble.
-  rewrite <- Nat.add_1_r in Hdouble.
-  exists p; assumption.
-Qed.
-
-Lemma nat_land_7_eq_intro:
-  forall n,
-  Nat.land n 7 = 7 -> exists m, n = 7 + 8 * m.
-Proof.
-  intros.
-  rewrite Nat.land_comm in H.
-  unfold Nat.land in H.
-  simpl in H.
-  destruct (Nat.odd n) eqn: Hodd.
-  - apply Hodd_spec in Hodd as Hn_eq.
-    destruct Hn_eq as (m & Hn_eq).
-    subst.
-    repeat rewrite Nat.add_0_r in H.
-    rewrite Nat.add_1_r in H.
-    repeat rewrite Div2.div2_double_plus_one in H.
-    destruct (Nat.odd m) eqn: Hoddm.
-    + apply Hodd_spec in Hoddm as Hm_eq.
-      destruct Hm_eq as (m0 & Hm_eq).
-      subst.
-      rewrite Nat.add_1_r in H.
-      repeat rewrite Div2.div2_double_plus_one in H.
-      destruct (Nat.odd m0) eqn: Hoddm0.
-      * apply Hodd_spec in Hoddm0 as Hm0_eq.
-        destruct Hm0_eq as (m & Hm_eq).
-        subst.
-        exists m.
-        lia.
-      * inversion H.
-    + rewrite Nat.add_0_l in H.
-      destruct (Nat.odd (Nat.div2 _)); inversion H.
-  - rewrite Nat.add_0_l in H.
-    repeat rewrite Nat.add_0_r in H.
-    rewrite <- Nat.negb_even in Hodd.
-    rewrite Bool.negb_false_iff in Hodd.
-    apply Heven_spec in Hodd as Hn_eq.
-    destruct Hn_eq as (m & Hn_eq).
-    subst.
-    repeat rewrite Div2.div2_double in H.
-    destruct (Nat.odd m) eqn: Hoddm.
-    + apply Hodd_spec in Hoddm as Hm_eq.
-      destruct Hm_eq as (m0 & Hm_eq).
-      subst.
-      rewrite Nat.add_1_r in H.
-      repeat rewrite Div2.div2_double_plus_one in H.
-      destruct (Nat.odd m0) eqn: Hoddm0.
-      * apply Hodd_spec in Hoddm0 as Hm0_eq.
-        destruct Hm0_eq as (m & Hm_eq).
-        subst.
-        exists m.
-        lia.
-      * inversion H.
-    + rewrite Nat.add_0_l in H.
-      destruct (Nat.odd (Nat.div2 _)); inversion H.
-Qed.
-
-Lemma nat_land_7_eq_elim:
-  forall n,
-  (exists m, n = 7 + 8 * m) -> Nat.land n 7 = 7.
-Proof.
-  intros.
-  destruct H as (m & H).
-  rewrite Nat.land_comm.
-  unfold Nat.land.
-  simpl.
-  subst.
-  rewrite Nat.odd_add.
-  change (Nat.odd 7) with true.
-  rewrite Nat.odd_mul.
-  change (Nat.odd 8) with false.
-  unfold xorb, andb.
-  assert (Heq: (7 + 8 * m) = (S (2 *(3+4*m)))) by lia.
-  rewrite Heq; clear Heq.
-  rewrite Div2.div2_double_plus_one.
-  rewrite Nat.odd_add.
-  change (Nat.odd 3) with true.
-  rewrite Nat.odd_mul.
-  change (Nat.odd 4) with false.
-  unfold xorb, andb.
-  assert (Heq: (3 + 4 * m) = (S (2 *(1+2*m)))) by lia.
-  rewrite Heq; clear Heq.
-  rewrite Div2.div2_double_plus_one.
-  rewrite Nat.odd_add.
-  change (Nat.odd 1) with true.
-  rewrite Nat.odd_mul.
-  change (Nat.odd 2) with false.
-  unfold xorb, andb.
-  lia.
-Qed.
-
-Lemma nat_land_7_eq:
-  forall n,
-    Nat.land n 7 = 7 <-> exists m, n = 7 + 8 * m.
-Proof.
-  intros.
-  split.
-  apply nat_land_7_eq_intro.
-  apply nat_land_7_eq_elim.
-Qed.
-
 Lemma nat_land_240_eq_128:
   forall n
     (Hrange : n <= 255)
@@ -641,7 +517,26 @@ Proof.
   - destruct H; subst; reflexivity.
 Qed.
 
+Lemma nat8_neq_k:
+  forall n k
+    (Hn_range : n <= 255)
+    (Hk_range : (0 <= k <= 255)%Z)
+    (Hc2_eq : (Z.of_nat n) <> k),
+      Int.repr (Z.of_nat n) <> Int.repr k.
+Proof.
+  repeat intro.
+  Transparent Int.repr.
+  unfold Int.repr in *.
+  inversion H.
+  rewrite Int.Z_mod_modulus_eq in H1.
+  rewrite Zmod_small in H1.
+  rewrite Int.Z_mod_modulus_eq in H1.
+  rewrite Zmod_small in H1.
+  lia.
+  all: change Int.modulus with 4294967296%Z; lia.
+Qed.
 
+(*
 Lemma nat8_neq_135:
   forall n
     (Hrange : n <= 255)
@@ -710,6 +605,7 @@ Proof.
   change Int.modulus with 4294967296%Z.
   lia.
 Qed.
+*)
 
 Lemma nat_odd_S:
   forall n,
@@ -725,19 +621,6 @@ Proof.
     rewrite Nat.odd_succ.
     rewrite Bool.negb_false_iff in Hodd.
     rewrite Hodd; reflexivity.
-Qed.
-
-Lemma Zland_0xff:
-  forall c
-    (Hc_le : c <= 255),
-      Nat.land c 255 = c.
-Proof.
-  intros.
-  assert (Hc: c < 256) by lia.
-  clear Hc_le.
-  do 255 (destruct c; [reflexivity |]).
-  destruct c; [reflexivity |].
-  destruct c;  lia.
 Qed.
 
 Ltac simpl_if Ht :=
